src/MicroSail/Symbolic/Sound.v
@@ -46,6 +46,9 @@ From MicroSail Require Import
      Tactics
      Symbolic.Mutator
      Symbolic.Outcome.
+From MicroSail Require
+     SemiConcrete.Mutator
+     SemiConcrete.Sound.
 
 Set Implicit Arguments.
 
@@ -62,6 +65,8 @@ Module Soundness
   Import MUT.
   Module LOG := ProgramLogic typekit termkit progkit assertkit contractkit.
   Import LOG.
+  Module SCMUT := SemiConcrete.Sound.Soundness typekit termkit progkit assertkit contractkit.
+  Import SCMUT.MUT.
 
   Program Instance proper_sub_comp {Σ1 Σ2 Σ3} : Proper (eq ==> eq ==> eq) (@sub_comp Σ1 Σ2 Σ3).
   Admit Obligations.
@@ -72,20 +77,330 @@ Module Soundness
 
     Section WithSemantics.
 
-      Context `{HL: IHeaplet L} {SLL: ISepLogicLaws L}.
-
-      Definition inst_heap {Σ} (ι : SymInstance Σ) (h : SymbolicHeap Σ) : L :=
-        List.fold_right (fun c h => inst_chunk ι c ∧ h) ltrue h.
-
       Axiom sub_comp_id_left : forall {Σ0 Σ1} (ζ : Sub Σ0 Σ1), sub_comp (sub_id Σ0) ζ = ζ.
       Axiom sub_comp_id_right : forall {Σ0 Σ1} (ζ : Sub Σ0 Σ1), sub_comp ζ (sub_id Σ1) = ζ.
       Axiom subst_sub_id : forall `{Subst T} Σ (t : T Σ), subst (sub_id _) t = t.
       Axiom subst_sub_comp : forall `{Subst T} Σ0 Σ1 Σ2 (ζ1 : Sub Σ0 Σ1) (ζ2 : Sub Σ1 Σ2) t, subst (sub_comp ζ1 ζ2) t = subst ζ2 (subst ζ1 t).
       Axiom sub_comp_comm : forall {Σ0 Σ1 Σ2 Σ3} (ζ1 : Sub Σ0 Σ1) (ζ2 : Sub Σ1 Σ2) (ζ3 : Sub Σ2 Σ3), sub_comp (sub_comp ζ1 ζ2) ζ3 = sub_comp ζ1 (sub_comp ζ2 ζ3).
 
-      (* Lemma  *)
-      (* subst ζ'' (symbolic_eval_exp δ0 e) *)
-      (* = symbolic_eval_exp (inst_localstore ζ'' δ0) *)
+      Definition concretize_heap {Σ} (ι : SymInstance Σ) (h : SymbolicHeap Σ) : SCHeap :=
+        List.map (inst_chunk ι) h.
+
+      Definition represents {Γ Σ} (ι : SymInstance Σ) (s__sym : SymbolicState Γ Σ) (s__sc : SCState Γ) : Prop :=
+        concretize_heap    ι (symbolicstate_heap s__sym)       = scstate_heap s__sc /\
+        inst_localstore    ι (symbolicstate_localstore s__sym) = scstate_localstore s__sc /\
+        inst_pathcondition ι (symbolicstate_pathcondition s__sym).
+
+      Definition syminstance_leq {Σ1 Σ2} (ζ : Sub Σ1 Σ2) (ι1 : SymInstance Σ1) (ι2 : SymInstance Σ2) : Prop :=
+        ι1 = env_map (fun _ => inst_term ι2) ζ.
+
+      Lemma syminstance_leq_refl {Σ} (ι : SymInstance Σ) :
+        syminstance_leq (sub_id Σ) ι ι.
+      Proof.
+        unfold SymInstance, NamedEnv, syminstance_leq, sub_id in *.
+        apply env_lookup_extensional.
+        intros [x τ] ?.
+        now rewrite env_map_tabulate, env_lookup_tabulate.
+      Qed.
+
+      Lemma syminstance_leq_snoc {Σ1 Σ2 x τ} (ζ : Sub Σ1 Σ2) (ι1 : SymInstance Σ1) ι2 :
+        forall v,
+          syminstance_leq ζ ι1 ι2 <->
+          syminstance_leq (env_snoc ζ (x,τ) (term_lit τ v)) (env_snoc ι1 (x,τ) v) ι2.
+      Proof.
+        unfold SymInstance, Sub, NamedEnv, syminstance_leq in *. intros. split.
+        - cbn; intros; subst; now cbn.
+        - cbn; intros.
+          now dependent elimination H.
+      Qed.
+
+      Definition scmut_wp {Γ1 Γ2 A}
+        (m : SCMut Γ1 Γ2 A)
+        (POST : A -> SCState Γ2 -> Prop)
+        (s1 : SCState Γ1) : Prop :=
+        outcome_satisfy (m s1) (fun r => POST (scmutres_value r) (scmutres_state r)).
+
+      Lemma scmut_wp_demonic_binary {Γ1 Γ2 A} (sm1 sm2 : SCMut Γ1 Γ2 A) (s__sc : SCState Γ1) (POST : A -> SCState Γ2 -> Prop) :
+        scmut_wp (scmut_demonic_binary sm1 sm2) POST s__sc <-> scmut_wp sm1 POST s__sc /\ scmut_wp sm2 POST s__sc.
+      Proof. unfold scmut_wp, scmut_demonic_binary; cbn; intuition. Qed.
+
+      Lemma scmut_wp_demonic {Γ1 Γ2 A B} (sm : B -> SCMut Γ1 Γ2 A) (s__sc : SCState Γ1) (POST : A -> SCState Γ2 -> Prop) :
+        scmut_wp (scmut_demonic sm) POST s__sc <-> forall v, scmut_wp (sm v) POST s__sc.
+      Proof. unfold scmut_wp, scmut_demonic; cbn; intuition. Qed.
+
+      Definition dmut_wp {Γ1 Γ2 Σ0 A}
+        (m : DynamicMutator Γ1 Γ2 A Σ0)
+        (POST : forall Σ1, Sub Σ0 Σ1 -> A Σ1 -> SymbolicState Γ2 Σ1 -> Prop)
+        (s1 : SymbolicState Γ1 Σ0) : Prop :=
+        forall Σ1 (ζ1 : Sub Σ0 Σ1),
+          outcome_satisfy
+            (m Σ1 ζ1 (subst ζ1 s1))
+            (fun '(@MkDynMutResult _ _ _ Σ2 ζ2 r) =>
+               POST
+                 Σ2
+                 (sub_comp ζ1 ζ2)
+                 (mutator_result_value r)
+                 (mutator_result_state r) /\
+               valid_obligations
+                 (mutator_result_obligations r)).
+
+      Lemma dmut_wp_demonic_binary {Γ1 Γ2 Σ A} (m1 m2 : DynamicMutator Γ1 Γ2 A Σ)
+        (POST : forall Σ', Sub Σ Σ' -> A Σ' -> SymbolicState Γ2 Σ' -> Prop) (s : SymbolicState Γ1 Σ) :
+          dmut_wp (dmut_demonic_binary m1 m2) POST s <->
+          dmut_wp m1 POST s /\ dmut_wp m2 POST s.
+      Proof. unfold dmut_wp, dmut_demonic_binary; cbn; intuition. Qed.
+
+      Lemma dmut_wp_demonic {Γ1 Γ2 Σ A B} (m : B -> DynamicMutator Γ1 Γ2 A Σ)
+        (POST : forall Σ', Sub Σ Σ' -> A Σ' -> SymbolicState Γ2 Σ' -> Prop) (s : SymbolicState Γ1 Σ) :
+          dmut_wp (dmut_demonic m) POST s <->
+          forall b, dmut_wp (m b) POST s.
+      Proof. unfold dmut_wp, dmut_demonic; cbn; intuition. Qed.
+
+      Lemma dmut_wp_fresh {Γ Σ0 A x τ}
+            (d : DynamicMutator Γ Γ A (Σ0 ▻ (x,τ))%ctx)
+            (POST : forall Σ1, Sub Σ0 Σ1 -> A Σ1 -> SymbolicState Γ Σ1 -> Prop)
+            (s : SymbolicState Γ Σ0) :
+        dmut_wp (dmut_fresh (x,τ) d) POST s <->
+        dmut_wp d (fun Σ1 ζ1 a1 s1 => POST Σ1 (env_tail ζ1) a1 s1) (wk1_symbolicstate s).
+      Proof.
+        unfold dmut_wp, dmut_fresh; cbn; split; intros HYP ? ?.
+        - dependent elimination ζ1 as [@env_snoc Σ0 ζ1 _ v]. cbn in v.
+          specialize (HYP Σ1 ζ1).
+          rewrite outcome_satisfy_map in HYP; cbn in *.
+          admit.
+        - specialize (HYP Σ1).
+          rewrite outcome_satisfy_map; cbn.
+          admit.
+      Admitted.
+
+      Lemma dmut_wp_fresh' {Γ Σ0 A x τ}
+            (d : DynamicMutator Γ Γ A (Σ0 ▻ (x,τ))%ctx)
+            (POST : forall Σ1, Sub Σ0 Σ1 -> A Σ1 -> SymbolicState Γ Σ1 -> Prop)
+            (s : SymbolicState Γ Σ0) :
+        dmut_wp (dmut_fresh (x,τ) d) POST s <->
+        forall v,
+          dmut_wp (dmut_sub (env_snoc (sub_id Σ0) (x,τ) (term_lit τ v)) d) POST s.
+      Proof.
+        unfold dmut_wp, dmut_fresh, dmut_sub; cbn. split; intro HYP.
+        - intros.
+          specialize (HYP Σ1 ζ1).
+          rewrite outcome_satisfy_map in HYP; cbn in *.
+          admit.
+        - intros ? ?.
+          rewrite outcome_satisfy_map.
+      Admitted.
+
+      Lemma dmut_wp_fresh_demonic {Γ Σ A x τ}
+            (d__d : Lit τ -> DynamicMutator Γ Γ A Σ)
+            (d__f : DynamicMutator Γ Γ A (Σ ▻ (x,τ))%ctx) :
+        (forall v POST s,
+            dmut_wp (d__d v) POST s <->
+            dmut_wp
+              (dmut_sub (env_snoc (sub_id Σ) (x,τ) (term_lit τ v)) d__f) POST s) ->
+        (forall
+            (POST : forall Σ', Sub Σ Σ' -> A Σ' -> SymbolicState Γ Σ' -> Prop)
+            (s : SymbolicState Γ Σ),
+            dmut_wp (dmut_fresh (x,τ) d__f) POST s <->
+            dmut_wp (dmut_demonic d__d) POST s).
+      Proof.
+        intros; split; intro HYP.
+        - apply dmut_wp_demonic. intros.
+          apply H. clear H. revert HYP. clear.
+          unfold dmut_wp, dmut_fresh, dmut_sub; cbn; intros.
+          specialize (HYP Σ1 ζ1).
+          rewrite outcome_satisfy_map in HYP.
+      Admitted.
+
+      Definition approximates {Γ1 Γ2 Σ} (ι : SymInstance Σ) (dm : DynamicMutator Γ1 Γ2 Unit Σ) (sm : SCMut Γ1 Γ2 unit) : Prop :=
+        forall (s__sym : SymbolicState Γ1 Σ) (s__sc : SCState Γ1) (POST : unit -> SCState Γ2 -> Prop),
+          represents ι s__sym s__sc ->
+          dmut_wp
+            dm
+            (fun Σ1 ζ1 v1 s__sym1 =>
+               forall ι1 s__sc1,
+                 syminstance_leq ζ1 ι ι1 ->
+                 represents ι1 s__sym1 s__sc1 ->
+                 POST v1 s__sc1)
+            s__sym ->
+          scmut_wp sm POST s__sc.
+
+      Lemma approximates_demonic_binary {Γ1 Γ2 Σ} (ι : SymInstance Σ)
+            (dm1 dm2 : DynamicMutator Γ1 Γ2 Unit Σ) (sm1 sm2 : SCMut Γ1 Γ2 unit) :
+        approximates ι dm1 sm1 ->
+        approximates ι dm2 sm2 ->
+        approximates ι (dmut_demonic_binary dm1 dm2) (scmut_demonic_binary sm1 sm2).
+      Proof.
+        intros H1 H2 ? ? ? H__s H.
+        apply scmut_wp_demonic_binary.
+        apply dmut_wp_demonic_binary in H.
+        split.
+        now apply (H1 _ _ _ H__s).
+        now apply (H2 _ _ _ H__s).
+      Qed.
+
+      Lemma dmut_produce_chunk_sound {Γ Σ} (ι : SymInstance Σ) (c : Chunk Σ) :
+        approximates
+          (Γ1 := Γ) (Γ2 := Γ) ι
+          (dmut_produce_chunk c)
+          (scmut_produce_chunk (inst_chunk ι c)).
+      Proof.
+        intros [pc δ__sym h__sym] [δ__sc h__sc] ? (H__h & H__δ & H__pc); cbn in *.
+        intros; destruct_conjs.
+        specialize (H Σ (sub_id Σ)). cbn in H.
+        destruct H as [H _]. apply (H ι); clear H.
+        rewrite sub_comp_id_left.
+        apply syminstance_leq_refl.
+        unfold represents; cbn.
+        now rewrite ?subst_sub_id, H__h.
+      Qed.
+
+      Lemma dmut_assume_term_sound {Γ Σ} (ι : SymInstance Σ) (b : Term Σ ty_bool) :
+        approximates
+          (Γ1 := Γ) (Γ2 := Γ) ι
+          (dmut_assume_term b)
+          (scmut_assume_term ι b).
+      Proof.
+        intros ? ? ? H__state H.
+        unfold dmut_wp, dmut_assume_term, dmut_assume_formula in H.
+        specialize (H Σ (sub_id Σ)).
+        change (sub_formula (sub_id Σ) (formula_bool b))
+          with (subst (sub_id Σ) (formula_bool b)) in H.
+        rewrite ?subst_sub_id in H.
+        destruct (try_solve_formula (formula_bool b)) as [[]|] eqn:?.
+        + unfold scmut_assume_term.
+          assert (inst_term ι b = true) as -> by admit.
+          cbn in H. destruct H as [H _].
+          cbn. apply (H ι).
+          * rewrite sub_comp_id_left.
+            apply syminstance_leq_refl.
+          * assumption.
+        + unfold scmut_assume_term.
+          assert (inst_term ι b = false) as -> by admit.
+          trivial.
+        + cbn in H. destruct H as [H _].
+          unfold scmut_assume_term.
+          destruct (inst_term ι b) eqn:?; cbn.
+          * apply (H ι).
+            rewrite sub_comp_id_left.
+            apply syminstance_leq_refl.
+            revert H__state Heql. clear.
+            unfold represents; destruct s__sym;
+              cbn; intuition.
+          * trivial.
+      Admitted.
+
+      Opaque dmut_assume_term.
+
+      Lemma dmut_fresh_sound {Γ Σ ς τ} (ι : SymInstance Σ)
+            (dm : DynamicMutator Γ Γ Unit (Σ ▻ (ς,τ)))
+            (sm : Lit τ -> SCMut Γ Γ unit) :
+        (forall v, approximates (env_snoc ι _ v) dm (sm v)) ->
+        approximates ι
+          (dmut_fresh (ς,τ) dm)
+          (scmut_demonic sm).
+      Proof.
+        intros HYP.
+        unfold approximates; cbn.
+        intros ? ? ? H__state H.
+        apply scmut_wp_demonic. intros v.
+        apply (HYP v (wk1_symbolicstate s__sym) s__sc POST).
+        - revert H__state. clear.
+          destruct s__sym, s__sc; unfold represents; cbn.
+          intros; destruct_conjs; repeat split.
+          + rewrite <- H. clear.
+            unfold subst, SubstList.
+            rewrite List.map_map.
+            apply List.map_ext.
+            intros.
+            admit.
+          + rewrite <- H0. clear.
+            unfold subst, sub_localstore.
+            rewrite env_map_map.
+            admit.
+          + revert H1; clear.
+            unfold subst, SubstList.
+            match goal with
+            | |- context[List.map ?f ?l] =>
+              change (List.map f l) with (base.fmap f l)
+            end.
+            rewrite list.foldr_fmap.
+            admit.
+        - (* unfold dmut_wp, dmut_fresh in *. *)
+          (* intros ? ?. *)
+          (* dependent elimination ζ1 as [@env_snoc Σ ζ1 _ v]. cbn in v. *)
+          (* specialize (H Σ1 ζ1). *)
+          (* rewrite outcome_satisfy_map in H. *)
+          apply (@dmut_wp_fresh Γ Σ Unit ς τ) in H.
+          (* rewrite syminstance_leq_snoc *)
+          (* apply H. *)
+      Admitted.
+
+      Lemma dmut_produce_sound {Γ Σ} (asn : Assertion Σ) (ι : SymInstance Σ) :
+        approximates
+          (Γ1 := Γ) (Γ2 := Γ) ι
+          (dmut_produce asn)
+          (scmut_produce ι asn).
+      Proof.
+        induction asn; cbn.
+        - apply dmut_assume_term_sound.
+        - admit. (* Not implemented in SC. OOPS *)
+        - apply dmut_produce_chunk_sound.
+        - enough
+            (approximates  (Γ1 := Γ) (Γ2 := Γ) ι
+               (dmut_demonic_binary
+                  (dmut_bind_right (dmut_assume_term b)            (dmut_produce asn1))
+                  (dmut_bind_right (dmut_assume_term (term_not b)) (dmut_produce asn2)))
+               (scmut_demonic_binary
+                  (scmut_bind_right (scmut_assume_term ι b)            (scmut_produce ι asn1))
+                  (scmut_bind_right (scmut_assume_term ι (term_not b)) (scmut_produce ι asn2)))) by admit.
+          apply approximates_demonic_binary.
+          + admit.
+          + admit.
+        - admit.
+        - admit.
+        - apply dmut_fresh_sound. intros. apply IHasn.
+      Admitted.
+
+      Opaque dmut_wp.
+      Opaque scmut_wp.
+
+      Context `{HL: IHeaplet L} {SLL: ISepLogicLaws L}.
+
+      Definition inst_heap {Σ} (ι : SymInstance Σ) (h : SymbolicHeap Σ) : L :=
+        List.fold_right (fun c h => ASS.inst_chunk ι c ∧ h) ltrue h.
+
+      (*   Definition rhoI {Γ Σ0} (ι0 : SymInstance Σ0) (s__sym : SymbolicState Γ Σ0) : *)
+      (*     Outcome (SCMutResult Γ { Σ : Ctx (𝑺 * Ty) & Sub Σ0 Σ * SymInstance Σ }%type) := *)
+      (*     ⨂ (Σ1 : Ctx (𝑺 * Ty)) *)
+      (*       (ζ1 : Sub Σ0 Σ1) *)
+      (*       (ι1 : SymInstance Σ1) *)
+      (*       (s__sc : SCState Γ) *)
+      (*       (_ : syminstance_leq ζ1 ι0 ι1) *)
+      (*       (_ : represents ι1 (subst ζ1 s__sym) s__sc) => *)
+      (*     outcome_pure *)
+      (*       {| scmutres_value := existT Σ1 (ζ1,ι1); *)
+      (*          scmutres_state := s__sc *)
+      (*       |}. *)
+      (* End Bla. *)
+
+      (* Definition approximates {Γ1 Γ2 Σ} (ι : SymInstance Σ) (dm : DynamicMutator Γ1 Γ2 Unit Σ) (sm : SCMut Γ1 Γ2 unit) : Prop. *)
+      (* Proof. *)
+      (*   refine ( *)
+      (*   forall s__sym : SymbolicState Γ1 Σ, *)
+      (*     outcome_cover *)
+      (*       (outcome_bind (dm Σ (sub_id _) s__sym) _) *)
+      (*       (outcome_bind (rhoI ι s__sym) (fun r__sc => sm (scmutres_state r__sc))) *)
+      (*     ). *)
+      (*   intros [Σ1 ζ1 [_ s__sym' x]]. *)
+      (*   eapply outcome_bind. *)
+      (*   eapply (rhoI ι). *)
+      (*   admit. *)
+      (*   intros [? s__sc']. *)
+      (*   apply outcome_pure. *)
+      (*   constructor. *)
+      (*   constructor. *)
+      (*   apply s__sc'. *)
+      (*   Show Proof. *)
 
       Ltac sauto :=
         repeat
@@ -154,123 +469,50 @@ Module Soundness
       Lemma dmut_exec_sound {Γ σ} (POST : Lit σ -> LocalStore Γ -> L) (s : Stm Γ σ) :
         forall Σ0 Σ1  (ι : SymInstance Σ1) (ζ1 : Sub Σ0 Σ1) (pc1 : PathCondition Σ1) (δ1 : SymbolicLocalStore Γ Σ1) (h1 : SymbolicHeap Σ1),
           let δ       := inst_localstore ι δ1 in
-          let pre__pc   := !! inst_pathcondition ι pc1 in
+          let pre__pc   := inst_pathcondition ι pc1 in
           let pre__heap := inst_heap ι h1 in
           outcome_satisfy
             (dmut_exec s ζ1 (MkSymbolicState pc1 δ1 h1))
             (fun '(@MkDynMutResult _ _ _ Σ2 ζ2 (MkMutResult t (MkSymbolicState pc2 δ2 h2) x)) =>
                forall (ι' : SymInstance Σ2),
                  ι = env_map (fun _ => inst_term ι') ζ2 ->
-                 let post__pc   := !! inst_pathcondition ι' pc2 in
+                 let post__pc   := inst_pathcondition ι' pc2 in
                  let post__heap := inst_heap ι' h2 in
-                 post__pc ∧ post__heap ⊢ POST (inst_term ι' t) (inst_localstore ι' δ2)) ->
-          δ ⊢ ⦃ pre__pc ∧ pre__heap ⦄ s ⦃ POST ⦄.
+                 !! post__pc ∧ post__heap ⊢ POST (inst_term ι' t) (inst_localstore ι' δ2)) ->
+          pre__pc ->
+          outcome_satisfy
+            (scmut_exec s (MkSCState δ (concretize_heap ι h1)))
+            (fun '(MkSCMutResult v2 (MkSCState δ2 h2)) =>
+               SCMUT.inst_scheap h2 ⊢ POST v2 δ2).
       Proof.
         intros ? ? ? ? ? ? ?; cbn.
         revert pc1 h1.
         induction s.
 
-        - intros.
-          apply rule_stm_lit.
-          apply H.
-          admit.
+        - cbn. intros.
+          assert (ι = env_map (fun b : 𝑺 * Ty => inst_term ι) (sub_id Σ1)) as Heqι by admit.
+          specialize (H ι Heqι); clear Heqι.
+          refine (entails_trans _ _ _ _ H).
+          apply land_right.
+          + now apply lprop_right.
+          + admit.
 
-        - intros.
-          apply rule_stm_exp.
+        - cbn. intros.
+          assert (ι = env_map (fun b : 𝑺 * Ty => inst_term ι) (sub_id Σ1)) as Heqι by admit.
+          specialize (H ι Heqι); clear Heqι.
           rewrite eval_exp_inst.
-          apply H.
-          admit.
+          refine (entails_trans _ _ _ _ H).
+          apply land_right.
+          + now apply lprop_right.
+          + admit.
 
-        - cbn.
-          unfold dmut_bind_right, dmut_sub, dmut_bind; cbn.
+        - repeat (unfold dmut_bind_right, dmut_sub, dmut_bind, scmut_bind,
+                  scmut_bind_left; cbn).
           repeat
             (repeat setoid_rewrite outcome_satisfy_bind;
              repeat setoid_rewrite outcome_satisfy_map; cbn).
-          repeat
-            (repeat setoid_rewrite sub_comp_id_left at 1;
-             repeat setoid_rewrite sub_comp_id_right at 1;
-             repeat setoid_rewrite subst_sub_id at 1;
-             cbn).
-          cbn.
           intros.
 
-          eapply rule_stm_let.
-          + apply IHs1.
-            refine (outcome_satisfy_monotonic _ _ H); clear H. intros ?.
-            unfold dmut_bind_right, dmut_sub, dmut_bind; cbn.
-            rewrite ?outcome_satisfy_bind, ?outcome_satisfy_map; cbn.
-            intros.
-            admit.
-          + admit.
-        - admit.
-        - admit.
-        - admit.
-        - admit.
-        - admit.
-        - cbn.
-          unfold dmut_bind_right, dmut_sub, dmut_bind; cbn.
-          repeat
-            (repeat setoid_rewrite outcome_satisfy_bind;
-             repeat setoid_rewrite outcome_satisfy_map; cbn).
-          repeat
-            (repeat setoid_rewrite sub_comp_id_left at 1;
-             repeat setoid_rewrite sub_comp_id_right at 1;
-             repeat setoid_rewrite subst_sub_id at 1;
-             cbn).
-          cbn.
-          cbv [mutator_assume_term mutator_assume_formula].
-          intros ? ? [H1 H2].
-          apply rule_stm_if.
-          + clear IHs2 H2.
-            revert H1.
-            destruct (try_solve_formula (formula_bool (symbolic_eval_exp δ1 e))) eqn:Heqfml.
-            * destruct (try_solve_formula_spec Term_eqb_spec (formula_bool (symbolic_eval_exp δ1 e)) Heqfml ι).
-              -- unfold mutator_pure; cbn.
-                 repeat
-                   (repeat setoid_rewrite outcome_satisfy_bind;
-                    repeat setoid_rewrite outcome_satisfy_map; cbn).
-                 repeat
-                   (repeat setoid_rewrite sub_comp_id_left at 1;
-                    repeat setoid_rewrite sub_comp_id_right at 1;
-                    repeat setoid_rewrite subst_sub_id at 1;
-                    cbn).
-                 intros H1.
-                 eapply rule_consequence; [ idtac | idtac | apply IHs1 ]; clear IHs1.
-                 apply land_left1. apply entails_refl.
-                 intros; apply entails_refl.
-                 admit.
-                 (* refine (outcome_satisfy_monotonic _ _ H1); clear H1. *)
-                 (* intros [Σ2 ζ2 [t2 [pc2 δ2 h2] oblig2]]; cbn; intros. *)
-                 (* apply H. *)
-                 (* now rewrite sub_comp_id_left. *)
-              -- intros H1; clear H1.
-                 cbn in n.
-                 unfold is_true in n.
-                 rewrite eval_exp_inst.
-                 destruct (inst_term ι (symbolic_eval_exp δ1 e)) eqn:?; try contradiction.
-                 clear n.
-                 clear Heqfml.
-                 admit.
-            * unfold mutator_modify, mutator_state; cbn.
-              repeat
-                (repeat setoid_rewrite outcome_satisfy_bind;
-                 repeat setoid_rewrite outcome_satisfy_map; cbn).
-              repeat
-                (repeat setoid_rewrite sub_comp_id_left at 1;
-                 repeat setoid_rewrite sub_comp_id_right at 1;
-                 repeat setoid_rewrite subst_sub_id at 1;
-                 cbn).
-              intro.
-              admit.
-              (* eapply rule_consequence; *)
-              (*   [ idtac *)
-              (*   | idtac *)
-              (*   | apply IHs1; refine (outcome_satisfy_monotonic _ _ H1) *)
-              (*   ]; clear H1 IHs1. *)
-              (* admit. *)
-              (* intros; apply entails_refl. *)
-              (* cbn. *)
-              (* intros [Σ2 ζ2 [t2 [pc2 δ2 h2] oblig2]]; cbn; intros. *)
       Admitted.
 
       Lemma dmut_contract_sound {Δ τ} (c : SepContract Δ τ) (body : Stm Δ τ) :
